some simp

Test.lean
@@ -1,4 +1,36 @@
 import Canonical.Main
 
-def test : 0 + n = n :=
-  by canonical [Nat.add_zero, Nat.add_succ]
+inductive MyNat
+| zero : MyNat
+| succ : MyNat → MyNat
+
+open MyNat
+
+def MyNat.add : MyNat → MyNat → MyNat
+| n, zero => n
+| n, succ m => succ (n.add m)
+
+theorem zero_add : zero.add n = n := by
+  exact
+    rec (motive := fun t ↦ zero.add t = t) (Eq.refl zero)
+      (fun a a_ih ↦
+        Eq.rec (motive := fun a_1 t ↦ (zero.add a).succ = a_1.succ) (Eq.refl (zero.add a).succ)
+          a_ih)
+      n
+
+theorem succ_add : (succ n).add m = succ (n.add m) := by
+  exact
+    rec (motive := fun t ↦ n.succ.add t = (n.add t).succ) (Eq.refl n.succ)
+      (fun a a_ih ↦
+        Eq.rec (motive := fun a_1 t ↦ (n.succ.add a).succ = a_1.succ) (Eq.refl (n.succ.add a).succ)
+          a_ih)
+      m
+
+theorem add_comm (n m : MyNat) : n.add m = m.add n := by
+  exact
+    rec (motive := fun t ↦ t.add m = m.add t)
+      (by simp only [MyNat.add.eq_1, zero_add] <;> exact Eq.refl m)
+      (by simp only [MyNat.succ.injEq, succ_add, MyNat.add.eq_2] <;> exact fun a a_ih ↦ a_ih) n
+
+
+def test (x : Nat) : 2^x = 2^x := by canonical
