Canonical/Simp.lean
@@ -1,0 +1,43 @@
+import Lean
+import Canonical.Util
+
+open Lean Meta Std DiscrTree Trie Key Expr
+
+namespace Canonical
+
+def SIMP_HARD_CODE : HashMap Name (Array Name) := .ofList [
+  (`Nat.succ_eq_add_one, #[`Nat.succ.injEq]),
+  (`Nat.add_zero, #[`Nat.add_zero, `Nat.add_succ, `Nat.succ_add, `Nat.add_assoc]),
+  (`Nat.mul_one, #[]),
+  (`Nat.one_mul, #[`Nat.succ_mul, `Nat.mul_assoc]),
+  (`Nat.one_pow, #[`Nat.pow_succ, `Nat.pow_add, `Nat.mul_pow]),
+  (`Nat.pow_one, #[]),
+]
+
+/-- Retrieves the `Origin`s in `trie` consisting only of constants in `constSet`.  -/
+partial def getOrigins (constSet : NameSet) (trie : Trie SimpTheorem) : Array Origin :=
+  match trie with
+  | node vs children =>
+    let filtered := children.filter fun child =>
+      match child.1 with
+      | .proj name _ _ | .const name _ => constSet.contains name
+      | .arrow => false
+      | _ => true
+    (vs.filterMap (fun x => if x.priority ≥ eval_prio default then some x.origin else none)) ++ filtered.flatMap (fun x => getOrigins constSet x.2)
+
+
+def getRelevantSimpTheorems (constSet : NameSet) : MetaM (Array Name) := do
+  let thms ← getSimpTheorems
+  let tries ← constSet.toArray.filterMapM fun x => do
+    pure (thms.post.root.find? (.const x (← typeArity1 (← getConstInfo x).type)))
+  let origins := tries.flatMap (getOrigins constSet)
+  let names := origins.filterMap fun x =>
+    if let .decl name _ _ := x then some name else none
+  let relevant ← names.filterM fun x => do
+    forallTelescopeReducing (← getConstInfo x).type fun _ body => do
+      if let some (_, lhs, _) := (eq? body) then do
+        (lhs.getUsedConstantsAsSet.diff constSet).foldM (fun acc name => do
+          pure (acc && (← getUnfoldableConst? name).isSome)
+        ) true
+      else pure false
+  pure (relevant.flatMap fun x => SIMP_HARD_CODE.getD x #[x])
